finish gluing model

theories/Core/Soundness/LogicalRelation.v
@@ -9,10 +9,10 @@ Global Open Scope predicate_scope.
 
 Generalizable All Variables.
 
-Notation "'typ_pred'" := (predicate (Tcons typ Tnil)).
-Notation "'glu_pred'" := (predicate (Tcons exp (Tcons typ (Tcons domain Tnil)))).
+Notation "'typ_pred'" := (predicate (Tcons ctx (Tcons typ Tnil))).
+Notation "'glu_pred'" := (predicate (Tcons ctx (Tcons exp (Tcons typ (Tcons domain Tnil))))).
 
-Definition univ_typ_pred Γ j i : typ_pred := fun T => {{ Γ ⊢ T ≈ Type@j :  Type@i }}.
+Definition univ_typ_pred j i : typ_pred := fun Γ T => {{ Γ ⊢ T ≈ Type@j :  Type@i }}.
 
 Inductive glu_nat : ctx -> exp -> domain -> Prop :=
 | glu_nat_zero :
@@ -27,53 +27,62 @@ Inductive glu_nat : ctx -> exp -> domain -> Prop :=
      (forall {Δ σ v}, {{ Δ ⊢w σ : Γ }} -> {{ Rne c in length Δ ↘ v }} -> {{ Δ ⊢ m [ σ ] ≈ v : ℕ }}) ->
      glu_nat Γ m d{{{ ⇑ ℕ c }}} ).
 
-Definition nat_typ_pred Γ i : typ_pred := fun M => {{ Γ ⊢ M ≈ ℕ :  Type@i }}.
+Definition nat_typ_pred i : typ_pred := fun Γ M => {{ Γ ⊢ M ≈ ℕ : Type@i }}.
 
-Definition nat_glu_pred Γ i : glu_pred := fun m M a => nat_typ_pred Γ i M /\ glu_nat Γ m a.
+Definition nat_glu_pred i : glu_pred := fun Γ m M a => nat_typ_pred i Γ M /\ glu_nat Γ m a.
 
-Definition neut_typ_pred Γ i C : typ_pred :=
-  fun M => {{ Γ ⊢ M : Type@i }} /\
+Definition neut_typ_pred i C : typ_pred :=
+  fun Γ M => {{ Γ ⊢ M : Type@i }} /\
           (forall Δ σ V, {{ Δ ⊢w σ : Γ }} -> {{ Rne C in length Δ ↘ V }} -> {{ Δ ⊢ M [ σ ] ≈ V : Type@i }}).
 
-Inductive neut_glu_pred Γ i C : glu_pred :=
-| ngp_make : forall m M A c,
-    neut_typ_pred Γ i C M ->
+Inductive neut_glu_pred i C : glu_pred :=
+| ngp_make : forall Γ m M A c,
+    neut_typ_pred i C Γ M ->
     per_bot c c ->
     (forall Δ σ V v, {{ Δ ⊢w σ : Γ }} ->
                 {{ Rne C in length Δ ↘ V }} ->
                 {{ Rne c in length Δ ↘ v }} ->
                 {{ Δ ⊢ m [ σ ] ≈ v : M [ σ ] }}) ->
-    neut_glu_pred Γ i C m M d{{{ ⇑ A c }}}.
+    neut_glu_pred i C Γ m M d{{{ ⇑ A c }}}.
 
-Inductive pi_typ_pred Γ i
+Inductive pi_typ_pred i
   (IR : relation domain)
   (IP : typ_pred)
   (IEl : glu_pred)
   (OP : forall c c' (equiv_c_c' : {{ Dom c ≈ c' ∈ IR }}),  typ_pred) : typ_pred :=
-| ptp_make : forall IT OT M,
+| ptp_make : forall Γ IT OT M,
     {{ Γ ⊢ M ≈ Π IT OT : Type@i }} ->
     {{ Γ , IT ⊢ OT : Type@i }} ->
-    (forall Δ σ, {{ Δ ⊢w σ : Γ }} -> IP {{{ IT [ σ ] }}}) ->
-    (forall Δ σ m a, {{ Δ ⊢w σ : Γ }} -> IEl m {{{ IT [ σ ] }}} a -> forall (Ha : IR a a), OP _ _ Ha {{{ OT [ σ ,, m ] }}}) ->
-    pi_typ_pred Γ i IR IP IEl OP M.
+    (forall Δ σ, {{ Δ ⊢w σ : Γ }} -> IP Δ {{{ IT [ σ ] }}}) ->
+    (forall Δ σ m a, {{ Δ ⊢w σ : Γ }} -> IEl Δ m {{{ IT [ σ ] }}} a -> forall (Ha : IR a a), OP _ _ Ha Δ {{{ OT [ σ ,, m ] }}}) ->
+    pi_typ_pred i IR IP IEl OP Γ M.
 
-Inductive pi_glu_pred Γ i
+Inductive pi_glu_pred i
   (IR : relation domain)
   (IP : typ_pred)
   (IEl : glu_pred)
-  (OP : forall c c' (equiv_c_c' : {{ Dom c ≈ c' ∈ IR }}),  typ_pred)
   (elem_rel : relation domain)
   (OEl : forall c c' (equiv_c_c' : {{ Dom c ≈ c' ∈ IR }}),  glu_pred): glu_pred :=
-| pgp_make : forall IT OT m M a,
+| pgp_make : forall Γ IT OT m M a,
     {{ Γ ⊢ m : M }} ->
     elem_rel a a ->
     {{ Γ ⊢ M ≈ Π IT OT : Type@i }} ->
     {{ Γ , IT ⊢ OT : Type@i }} ->
-    (forall Δ σ, {{ Δ ⊢w σ : Γ }} -> IP {{{ IT [ σ ] }}}) ->
-    (forall Δ σ m' b, {{ Δ ⊢w σ : Γ }} -> IEl m' {{{ IT [ σ ] }}} b -> forall (Ha : IR b b),
-    exists ab, {{ $| a & b |↘ ab }} /\ OEl _ _ Ha {{{ m [ σ ] m' }}} {{{ OT [ σ ,, m' ] }}} ab) ->
-    pi_glu_pred Γ i IR IP IEl OP elem_rel OEl m M a.
+    (forall Δ σ, {{ Δ ⊢w σ : Γ }} -> IP Δ {{{ IT [ σ ] }}}) ->
+    (forall Δ σ m' b, {{ Δ ⊢w σ : Γ }} -> IEl Δ m' {{{ IT [ σ ] }}} b -> forall (Ha : IR b b),
+    exists ab, {{ $| a & b |↘ ab }} /\ OEl _ _ Ha Δ {{{ m [ σ ] m' }}} {{{ OT [ σ ,, m' ] }}} ab) ->
+    pi_glu_pred i IR IP IEl elem_rel OEl Γ m M a.
 
+
+Lemma pi_glu_pred_pi_typ_pred : forall i IR IP IEl (OP : forall c c' (equiv_c_c' : {{ Dom c ≈ c' ∈ IR }}),  typ_pred) elem_rel OEl Γ m M a,
+    pi_glu_pred i IR IP IEl elem_rel OEl Γ m M a ->
+    (forall Δ m' M' b c c' (Hc : IR c c'), OEl _ _ Hc Δ m' M' b -> OP _ _ Hc Δ M') ->
+    pi_typ_pred i IR IP IEl OP Γ M.
+Proof.
+  inversion_clear 1; econstructor; eauto.
+  intros.
+  edestruct H5 as [? []]; eauto.
+Qed.
 
 Section Gluing.
   Variable
@@ -81,13 +90,13 @@ Section Gluing.
       (glu_univ_rec : forall {j}, j < i -> relation domain)
       (glu_univ_typ_rec : forall {j}, j < i -> typ_pred).
 
-  Definition univ_glu_pred Γ {j} (lt_j_i : j < i) : glu_pred :=
-    fun m M A =>
+  Definition univ_glu_pred {j} (lt_j_i : j < i) : glu_pred :=
+    fun Γ m M A =>
     {{ Γ ⊢ m : M }} /\ {{ Γ ⊢ M ≈ Type@j : Type@i }} /\
       glu_univ_rec lt_j_i A A /\
-      glu_univ_typ_rec lt_j_i m.
+      glu_univ_typ_rec lt_j_i Γ m.
 
-  Inductive glu_univ_elem_core : ctx -> typ_pred -> glu_pred -> relation domain -> domain -> domain -> Prop :=
+  Inductive glu_univ_elem_core : typ_pred -> glu_pred -> relation domain -> domain -> domain -> Prop :=
   | glu_univ_elem_core_univ :
     `{ forall (elem_rel : relation domain)
          typ_rel
@@ -95,38 +104,43 @@ Section Gluing.
          (lt_j_i : j < i),
           j = j' ->
           (elem_rel <~> glu_univ_rec lt_j_i) ->
-          typ_rel <∙> univ_typ_pred Γ j i ->
-          el_rel <∙> univ_glu_pred Γ lt_j_i ->
-          glu_univ_elem_core Γ typ_rel el_rel elem_rel d{{{ 𝕌@j }}} d{{{ 𝕌@j' }}} }
+          typ_rel <∙> univ_typ_pred j i ->
+          el_rel <∙> univ_glu_pred lt_j_i ->
+          glu_univ_elem_core typ_rel el_rel elem_rel d{{{ 𝕌@j }}} d{{{ 𝕌@j' }}} }
 
   | glu_univ_elem_core_nat :
     `{ forall (elem_rel : relation domain)
          typ_rel el_rel,
           (elem_rel <~> per_nat) ->
-          typ_rel <∙> nat_typ_pred Γ i ->
-          el_rel <∙> nat_glu_pred Γ i ->
-          glu_univ_elem_core Γ nat_rel el_rel elem_rel d{{{ ℕ }}} d{{{ ℕ }}} }
+          typ_rel <∙> nat_typ_pred i ->
+          el_rel <∙> nat_glu_pred i ->
+          glu_univ_elem_core nat_rel el_rel elem_rel d{{{ ℕ }}} d{{{ ℕ }}} }
 
-  (* | glu_univ_elem_core_pi : *)
-  (*   `{ forall (in_rel : relation domain) *)
-  (*        IP IEl *)
-  (*        (out_rel : forall {c c'} (equiv_c_c' : {{ Dom c ≈ c' ∈ in_rel }}), relation domain) *)
-  (*        typ_rel el_rel *)
-  (*        (elem_rel : relation domain), *)
-  (*         glu_univ_elem_core Γ in_rel IP IEl a a' -> *)
-  (*         (forall {c c'} (equiv_c_c' : {{ Dom c ≈ c' ∈ in_rel }}), *)
-  (*             rel_mod_eval per_univ_elem_core B d{{{ p ↦ c }}} B' d{{{ p' ↦ c' }}} (out_rel equiv_c_c')) -> *)
-
-  (*         (elem_rel <~> fun f f' => forall c c' (equiv_c_c' : {{ Dom c ≈ c' ∈ in_rel }}), rel_mod_app f c f' c' (out_rel equiv_c_c')) -> *)
-  (*         glu_univ_elem_core Γ typ_rel el_rel elem_rel d{{{ Π a p B }}} d{{{ Π a' p' B' }}} } *)
+  | glu_univ_elem_core_pi :
+    `{ forall (in_rel : relation domain)
+         IP IEl
+         (out_rel : forall {c c'} (equiv_c_c' : {{ Dom c ≈ c' ∈ in_rel }}), relation domain)
+         (OP : forall c c' (equiv_c_c' : {{ Dom c ≈ c' ∈ in_rel }}), typ_pred)
+         (OEl : forall c c' (equiv_c_c' : {{ Dom c ≈ c' ∈ in_rel }}), glu_pred)
+         typ_rel el_rel
+         (elem_rel : relation domain),
+          glu_univ_elem_core IP IEl in_rel a a' ->
+          (forall {c c'} (equiv_c_c' : {{ Dom c ≈ c' ∈ in_rel }}),
+              rel_mod_eval (glu_univ_elem_core (OP _ _ equiv_c_c') (OEl _ _ equiv_c_c'))
+                B d{{{ p ↦ c }}} B' d{{{ p' ↦ c' }}}
+                (out_rel equiv_c_c')) ->
+          (elem_rel <~> fun f f' => forall c c' (equiv_c_c' : {{ Dom c ≈ c' ∈ in_rel }}), rel_mod_app f c f' c' (out_rel equiv_c_c')) ->
+          typ_rel <∙> pi_typ_pred i in_rel IP IEl OP ->
+          el_rel <∙> pi_glu_pred i in_rel IP IEl elem_rel OEl ->
+          glu_univ_elem_core typ_rel el_rel elem_rel d{{{ Π a p B }}} d{{{ Π a' p' B' }}} }
 
   | glu_univ_elem_core_neut :
     `{ forall (elem_rel : relation domain)
          typ_rel el_rel,
           {{ Dom b ≈ b' ∈ per_bot }} ->
           (elem_rel <~> per_ne) ->
-          typ_rel <∙> neut_typ_pred Γ i b ->
-          el_rel <∙> neut_glu_pred Γ i b ->
-          glu_univ_elem_core Γ typ_rel el_rel elem_rel d{{{ ⇑ a b }}} d{{{ ⇑ a' b' }}} }.
+          typ_rel <∙> neut_typ_pred i b ->
+          el_rel <∙> neut_glu_pred i b ->
+          glu_univ_elem_core typ_rel el_rel elem_rel d{{{ ⇑ a b }}} d{{{ ⇑ a' b' }}} }.
 
 End Gluing.
